LeanScratch/Graph.lean
@@ -1,0 +1,35 @@
+import Mathlib.Data.Rel
+
+abbrev Graph α := Rel α α
+
+namespace Graph
+
+structure Path (α : Type*) :=
+  selector : ℕ → Option α
+  terminal : ∀ n, selector n = none → selector n.succ = none
+
+def Path.shorten (x : Path α) : Path α where
+  selector n := x.selector n.succ
+  terminal n w := x.terminal (n + 1) w
+
+abbrev FinPath := List
+
+def Path.IsFin (x : Path α) := ∃ n, x.selector n = .none
+
+inductive Path.length : Path α → ℕ → Prop
+  | zero : p.selector 0 = .none → length p 0
+  | cont { p : Path α } : (∃ v, p.selector 0 = .some v) → length p.shorten l → length p l.succ
+
+def Path.length' (p : Path α) (h : Path.IsFin p) : ℕ :=
+  let ⟨w, p⟩ := h
+  sorry
+
+/- #check Equiv -/
+
+namespace Path
+
+end Path
+
+def Acyclic (g : Graph α) : Prop := ¬∃ x, Relation.TransGen g x x
+
+
