LeanScratch/Semantics/STLC.lean
@@ -1,3 +1,4 @@
 import LeanScratch.Semantics.STLC.Stx
 import LeanScratch.Semantics.STLC.Red
 import LeanScratch.Semantics.STLC.Typed
+import LeanScratch.Semantics.STLC.StrongNorm
