LeanScratch/Semantics/STLC/StrongNorm.lean
@@ -1,0 +1,415 @@
+import LeanScratch.Semantics.STLC.Stx
+import LeanScratch.Semantics.STLC.Red
+import LeanScratch.Semantics.STLC.Typed
+import LeanScratch.Semantics.STLC.Infer
+import LeanScratch.ListUtils
+
+/-
+
+# Possible ways to solve strong normalization of STLC
+
+What does it mean for something to happen 'eventually'
+
+1.  [ ] Encode terms as ordinals
+2.  [ ] Simple structural recursion
+3.  [ ] Number of unique types decrease
+4.  [ ] Encode problem as a graph, prove there are no infinite paths + cycles
+5.  [ ] Number of bound variables
+6.  [ ] Number of lambdas
+7.  [ ] Maximum bound variable decreases (eventually?)
+8.  [ ] Locations where a function can be applied decreases
+9.  [ ] Any of the above apply on a congruence level - what does this mean
+10. [ ] A solution either decreases the maximum bvar, or it removes one bvar below it
+11. [ ] 'Negative bvars' are bound variables simply used within an
+        expression, number of 'negative bvars decrease'
+12. [ ] Do any of these metrics even matter on an application level?
+13. [ ] Eventually the smallest negative bvar has to be reduced
+14. [ ] A vector of negative bvars and occurances of said negative bvars decrease
+15. [ ] The negative bvar vector looks like a CNF-ordinal
+16. [ ] The types get less arrows in them in total
+17. [ ] The level of congruance application (eventually) decreases this relates
+18. [ ] Either types will stick around, or they will (eventually) be removed
+19. [ ] Types of lambdas cannot be created, only destroyed
+20. [ ] Number of 'hot applications' decreases, number of applications
+        with a lambda at some point on the left
+21. [ ] If any of the above hold for any sub-expression (like a lhs)
+        and for a (rhs) we can dictate they might hold for the whole expr
+22. [ ] Reducability decrease, this tracks how many lambdas / bvars
+        are on the left hand side of an expression
+23. [ ] 
+24. [ ] 
+25. [ ] 
+26. [ ] 
+27. [ ] 
+
+-/
+
+namespace STLC
+
+/- inductive TypeCount (t : Ty) : List Ty → Stx → ℕ → Prop -/
+/-   | absEq  : TypeCount t (t :: ls)  body n            → TypeCount t ls (.abs t body ) n.succ -/
+/-   | absNeq : t' ≠ t → TypeCount t (t' :: ls) body n   → TypeCount t ls (.abs t' body) n -/
+/-   | app  : TypeCount t ls a n → TypeCount t ls b k    → TypeCount t ls (.app a b) (n + k) -/
+/-   | beq  : ls[i]? = .some t                           → TypeCount t ls (.bvar i) 1 -/
+/-   | bneq : ls[i]? ≠ .some t                           → TypeCount t ls (.bvar i) 0 -/
+
+/- def typeCount (t : Ty) (ls : List Ty) : Stx → ℕ -/
+/-   | .abs ty body => (typeCount t (ty :: ls) body) + (if ty = t then 1 else 0) -/
+/-   | .app a b => (typeCount t ls a) + (typeCount t ls b) -/
+/-   | .bvar i => if ls[i]? = .some t then 1 else 0 -/
+
+/- theorem typeCount_TypeCount : typeCount t ls s = n ↔ TypeCount t ls s n := match s with -/
+/-   | .abs ty body => by -/
+/-     constructor -/
+/-     <;> intro h -/
+/-     · dsimp [typeCount] at h -/
+/-       split at h -/
+/-       next hz => -/
+/-         obtain ⟨w, p⟩ : ∃ n', typeCount t (ty :: ls) body = n' := exists_eq' -/
+/-         rw [p ] at h -/
+/-         rw [hz] at p ⊢ -/
+/-         rw [←h] -/
+/-         exact .absEq (typeCount_TypeCount.mp p) -/
+/-       next hz => exact .absNeq hz (typeCount_TypeCount.mp h) -/
+/-     · rcases h with (h|h) -/
+/-       · rename_i n -/
+/-         simp only [typeCount, ↓reduceIte, Nat.succ_eq_add_one, add_left_inj] -/
+/-         exact typeCount_TypeCount.mpr h -/
+/-       next hz => -/
+/-         simp [typeCount] -/
+/-         split -/
+/-         · contradiction -/
+/-         · dsimp -/
+/-           exact typeCount_TypeCount.mpr hz -/
+/-   | .app a b => by -/
+/-     constructor -/
+/-     <;> intro h -/
+/-     · dsimp [typeCount] at h -/
+/-       obtain ⟨an, ap⟩ : ∃ n', typeCount t ls a = n' := exists_eq' -/
+/-       obtain ⟨bn, bp⟩ : ∃ k', typeCount t ls b = k' := exists_eq' -/
+/-       rw [ap, bp] at h -/
+/-       rw [←h] -/
+/-       exact .app (typeCount_TypeCount.mp ap) (typeCount_TypeCount.mp bp) -/
+/-     · cases h -/
+/-       next n k a b => -/
+/-       dsimp [typeCount] -/
+/-       rw [(typeCount_TypeCount).mpr a, typeCount_TypeCount.mpr b] -/
+/-   | .bvar id => by -/
+/-     constructor -/
+/-     <;> intro h -/
+/-     · dsimp [typeCount] at h -/
+/-       split at h -/
+/-       <;> rw [←h] -/
+/-       next hz => exact .beq  hz -/
+/-       next hz => exact .bneq hz -/
+/-     · cases h <;> simpa [typeCount] -/
+
+namespace Counting
+
+inductive TypeCount (t : Ty) : List Ty → Stx → ℕ → Prop
+  | absEq  : TypeCount t (t :: ls)  body n            → TypeCount t ls (.abs t body ) n.succ
+  | absNeq : t' ≠ t → TypeCount t (t' :: ls) body n   → TypeCount t ls (.abs t' body) n
+  | app  : TypeCount t ls a n → TypeCount t ls b k    → TypeCount t ls (.app a b) (n + k)
+  | bvar :                                              TypeCount t ls (.bvar i) 0
+
+def typeCount (t : Ty) (ls : List Ty) : Stx → ℕ
+  | .abs ty body => (typeCount t (ty :: ls) body) + (if ty = t then 1 else 0)
+  | .app a b => (typeCount t ls a) + (typeCount t ls b)
+  | .bvar _ => 0
+
+theorem typeCount_TypeCount : typeCount t ls s = n ↔ TypeCount t ls s n := match s with
+  | .abs ty body => by
+    constructor
+    <;> intro h
+    · dsimp [typeCount] at h
+      split at h
+      next hz =>
+        obtain ⟨w, p⟩ : ∃ n', typeCount t (ty :: ls) body = n' := exists_eq'
+        rw [p ] at h
+        rw [hz] at p ⊢
+        rw [←h]
+        exact .absEq (typeCount_TypeCount.mp p)
+      next hz => exact .absNeq hz (typeCount_TypeCount.mp h)
+    · rcases h with (h|h)
+      · rename_i n
+        simp only [typeCount, ↓reduceIte, Nat.succ_eq_add_one, add_left_inj]
+        exact typeCount_TypeCount.mpr h
+      next hz =>
+        dsimp [typeCount]
+        split
+        · contradiction
+        · dsimp
+          exact typeCount_TypeCount.mpr hz
+  | .app a b => by
+    constructor
+    <;> intro h
+    · dsimp [typeCount] at h
+      obtain ⟨an, ap⟩ : ∃ n', typeCount t ls a = n' := exists_eq'
+      obtain ⟨bn, bp⟩ : ∃ k', typeCount t ls b = k' := exists_eq'
+      rw [ap, bp] at h
+      rw [←h]
+      exact .app (typeCount_TypeCount.mp ap) (typeCount_TypeCount.mp bp)
+    · cases h
+      next n k a b =>
+      dsimp [typeCount]
+      rw [(typeCount_TypeCount).mpr a, typeCount_TypeCount.mpr b]
+  | .bvar id => by
+    constructor
+    <;> intro h
+    · dsimp [typeCount] at h
+      rw [←h]
+      exact .bvar
+    · cases h
+      dsimp [typeCount]
+
+inductive BvarArity : ℕ → Stx → ℕ → Prop
+  | bvarEq  :                                       BvarArity i (.bvar i) 1
+  | bvarNeq : i ≠ j                               → BvarArity i (.bvar j) 0
+  | app     : BvarArity i a n → BvarArity i b k   → BvarArity i (.app a b) (n + k)
+  | abs     : BvarArity i.succ body n             → BvarArity i (.abs _ body) n
+
+def bvarArity (i : ℕ) : Stx → ℕ
+  | .abs _ body => bvarArity i.succ body
+  | .app a b => (bvarArity i a) + (bvarArity i b)
+  | .bvar j => if i = j then 1 else 0
+
+theorem bvarArity_BvarArity : bvarArity i s = n ↔ BvarArity i s n := match s with
+  | .abs ty body => by
+    constructor
+    <;> intro h
+    · dsimp [bvarArity] at h
+      exact .abs (bvarArity_BvarArity.mp h)
+    · dsimp [bvarArity]
+      rcases h with (_|_|_|h)
+      exact bvarArity_BvarArity.mpr h
+  | .app a b => by
+    constructor
+    <;> intro h
+    · dsimp [bvarArity] at h
+      obtain ⟨an, ap⟩ : ∃ n', bvarArity i a = n' := exists_eq'
+      obtain ⟨bn, bp⟩ : ∃ k', bvarArity i b = k' := exists_eq'
+      rw [ap, bp] at h
+      rw [←h]
+      exact .app (bvarArity_BvarArity.mp ap) (bvarArity_BvarArity.mp bp)
+    · dsimp [bvarArity]
+      cases h
+      next n' k' a b=>
+      rw [←bvarArity_BvarArity.mpr a, ←bvarArity_BvarArity.mpr b]
+  | .bvar j => by
+    constructor
+    <;> intro h
+    · dsimp [bvarArity] at h
+      split at h
+      next hz =>
+        rw [←h, hz]
+        exact .bvarEq
+      next hz =>
+        rw [←h]
+        exact .bvarNeq hz
+    · rcases h with (_|h)
+      <;> simp only [bvarArity, ite_eq_right_iff, one_ne_zero, imp_false, ↓reduceIte]
+      exact h
+
+end Counting
+
+namespace Bounding1
+/-
+  max ((λ x. $0) $1) f =>
+    let a := max $1 f
+    max $0
+-/
+
+def ArgCount : Ty → Type
+  | .arr a b  => ArgCount a → ArgCount b
+  | .direct _ => ℕ
+
+inductive TyArr : List Ty → Type
+  | nil : TyArr []
+  | cons (h : ArgCount hd) (t : TyArr tl) : TyArr (hd :: tl)
+
+namespace TyArr
+
+def get
+    {idx : ℕ} (h : Γ[idx]? = some ty) (v : TyArr Γ)
+    : ArgCount ty := match Γ, idx with
+  | [], _ => Option.noConfusion (cast (by rw [List.getElem?_nil]) h)
+  | hd :: tl, 0 =>
+    let h := cast (by rw [List.getElem?_cons_zero, Option.some.injEq]) h
+    match v with
+    | .cons hd _ => cast (by rw [←h]) hd
+  | hd :: tl, n+1 =>
+    let h := cast (by rw [List.getElem?_cons_succ]) h
+    match v with | cons _ tl' => get h tl'
+
+end TyArr
+
+namespace ArgCount
+
+def inc (h : ArgCount v) : ArgCount v := match v with
+  | .direct _ => Nat.succ h
+  | .arr _ _ => fun a' => inc (h a')
+
+theorem inferTyTransform
+    (h : infer Γ (.app a b) = some rTy)
+    (ha : infer Γ a = some aTy) (hb : infer Γ b = some bTy)
+    : aTy = .arr bTy rTy := by
+  simp only [infer, ha, hb, Option.bind_eq_bind, Option.some_bind] at h
+  split at h
+  <;> (try split at h)
+  <;> (try contradiction)
+  next h' =>
+  rw [(Option.some.injEq _ _).mp h, h']
+
+/--
+  This is a function that extracts the type that's an argument to the application.
+  This has to be done with a Σ' type over an ∃ because `Prop` can't be elim'd into `Type*`.
+  That being said its output is exacly the same as if it was done with ∃.
+-/
+def inferExtract
+    (h : infer Γ (.app a b) = some rTy)
+    : (aTy : Ty) ×' (infer Γ a = (aTy ⇒ rTy) ∧ infer Γ b = aTy) :=
+  match ha : infer Γ a, hb : infer Γ b with
+  | some aTy, some bTy  =>
+    ⟨_, Option.some_inj.mpr $ inferTyTransform h ha hb, rfl⟩
+  | none, _ => by
+    -- contra
+    simp only [infer, ha, Option.bind_eq_bind, Option.none_bind] at h
+  | some (.direct _), none
+  | some (.arr _ _),  none => by
+    simp only [infer, ha, hb, Option.bind_eq_bind, Option.none_bind, Option.some_bind] at h
+
+set_option trace.split.failure true in
+set_option pp.proofs true in
+theorem inferExtract_def
+    (h : infer Γ (.app a b) = some rTy)
+    : ∃ aTy, ∃ p₁, ∃ p₂, inferExtract h = ⟨aTy, p₁, p₂⟩ := by
+  rcases TySpec_app.mp (infer_TySpec.mp h) with ⟨argTy, p₁, p₂⟩
+  have p₁ := infer_TySpec.mpr p₁
+  have p₂ := infer_TySpec.mpr p₂
+  use argTy
+  use p₁
+  use p₂
+  dsimp [inferExtract]
+  split
+  /- · sorry -/
+  /- · sorry -/
+  /- · sorry -/
+  /- · sorry -/
+
+#print inferExtract
+
+-- I finally see why proof-relevance is useful.
+-- Damn that took me a long time to get
+-- This does not work due to how AC is defined on Prop...
+-- And (=) does only produce a Prop
+
+theorem inferFwd : infer Γ (Stx.abs argTy body) = some (.arr argTy' retTy)
+    → infer (argTy :: Γ) body = some retTy ∧ argTy = argTy' := by
+  simp only [infer, Option.map_eq_some', Ty.arr.injEq, exists_eq_right_right, imp_self]
+
+def upperBoundRed
+    {x : Stx} (hTy : infer Γ x = some ty)
+    (v : TyArr Γ)
+    : ArgCount ty := match x, ty with
+  | .bvar idx, _ => TyArr.get hTy v
+  | .abs argTy body, .arr argTy' retTy =>
+    let ⟨a, rfl⟩ := inferFwd hTy
+    fun z => upperBoundRed a (.cons z v)
+  | .abs argTy body, .direct _ => by
+    -- contra
+    simp only [infer, Option.map_eq_some', and_false, exists_false] at hTy
+  | .app a b, _ =>
+    let ⟨_, ha, hb⟩ := inferExtract hTy
+    ArgCount.inc $ (upperBoundRed ha v) (upperBoundRed hb v)
+
+def zero : ArgCount v := match v with
+  | .direct _ => Nat.zero
+  | .arr _ _ => fun _ => ArgCount.zero
+def naturalize (h : ArgCount v) : ℕ := match v with
+  | .direct _ => h
+  | .arr _ _ => naturalize (h ArgCount.zero)
+
+theorem naturalize_zero : naturalize (@zero v) = 0 := match v with
+  | .direct _ => rfl
+  | .arr _ _ => by dsimp [naturalize]; exact naturalize_zero
+
+theorem naturalize_inc
+    (x : ArgCount z)
+    : (naturalize x) + 1 = naturalize (inc x) :=
+  match z with
+  | .direct _ => rfl
+  | .arr _ _ => by simp only [naturalize, naturalize_inc, inc]
+
+/- def lt (a b : ArgCount v) : Prop := match v with -/
+/-   | .direct _ => Nat.lt a b -/
+/-   | .arr arg _ => ∀ z : ArgCount arg, ArgCount.lt (a z) (b z) -/
+
+/- theorem upperBoundRed_lt_inc -/
+/-     {p : infer Γ x = some t} -/
+/-     (h : upperBoundRed p Γ' = v) -/
+/-     : ArgCount.lt v v.inc := match t with -/
+/-     | .direct _ => by -/
+/-       simp only [ArgCount.lt, ArgCount.inc, Nat.succ_eq_add_one, Nat.lt_eq, lt_add_iff_pos_right, -/
+/-         zero_lt_one] -/
+/-     | .arr a b => by -/
+/-       intro z -/
+/-       simp [ArgCount.lt, ArgCount.inc] -/
+/-       sorry -/
+
+end ArgCount
+
+/- open ArgCount in -/
+/- theorem z (h : infer Γ s = some v) : inferExtract p = ⟨_, _, _⟩ := sorry -/
+
+open ArgCount in
+theorem β_naturalize
+    {p₁ : infer Γ (.app (.abs argTy body) arg) = some t₁}
+    {p₂ : infer Γ (body.β arg) = some t₁}
+    (h₁ : upperBoundRed p₁ Γ' = acA)
+    (h₂ : upperBoundRed p₂ Γ' = acB)
+    : naturalize acB < naturalize acA :=
+  match body with
+  | .abs argTy₂ b₂ => by
+    obtain (_|(_|(_|_))) := infer_TySpec.mp p₁
+    next p₁₁ p₁₂ =>
+    cases p₁₂
+    next p₁₂ =>
+    let this := infer_TySpec.mpr p₁₂
+    simp [upperBoundRed] at h₁
+    simp [inferExtract] at h₁
+    sorry
+  | .bvar idx => by
+    sorry
+  | .app a b => sorry
+
+end Bounding1
+
+
+namespace Bounding2
+
+-- C for constructive
+inductive CTySpec : List Ty → Stx → Ty → Type
+  | bvar ty : Γ[idx]? = some ty → CTySpec Γ (.bvar idx) ty
+
+  | app argTy retTy : CTySpec Γ fn (argTy ⇒ retTy) → CTySpec Γ arg argTy
+      → CTySpec Γ (.app fn arg) retTy
+  | abs argTy retTy : CTySpec (argTy :: Γ) body retTy
+      → CTySpec Γ (.abs ty body) (argTy ⇒ retTy)
+
+def build (h : infer Γ s = some ty) : CTySpec Γ s ty :=
+  match s with
+  | .bvar idx => .bvar _ (by simpa only)
+  | .abs ty body =>
+    match h' : infer (ty :: Γ) body with
+    | .none => by
+      -- contra
+      simp [infer, h'] at h
+    | .some x => by
+      simp only [infer, h', Option.map_some', Option.some.injEq] at h
+      subst h
+      exact .abs _ _ (build h')
+  | .app a b =>
+    have := Bounding1.inferExtract
+    sorry
+
+end Bounding2
